leader and learner message invariants

networkInvariantPrototypes/paxos/proof.dfy
@@ -11,6 +11,7 @@ module PaxosProof {
   ***************************************************************************************/
 
   // certified self-inductive
+  // Every message in the network has a valid source
   predicate ValidMessageSrc(c: Constants, v: Variables) 
     requires v.WF(c)
   {
@@ -18,16 +19,60 @@ module PaxosProof {
     :: 
     match msg 
       case Prepare(bal) => c.ValidLeaderIdx(bal)
-      case Promise(bal, acc, _) => c.ValidLeaderIdx(bal) && c.ValidAcceptorIdx(acc)
+      case Promise(_, acc, _) => c.ValidAcceptorIdx(acc)
       case Propose(bal, _) => c.ValidLeaderIdx(bal)
       case Accept(_, acc) => c.ValidAcceptorIdx(acc)
       case Learn(_) => true
+  }
+
+  // certified self-inductive
+  // Leader updates its highestHeard and value based on a Promise message carrying that
+  // ballot and value
+  predicate LeaderValidHighestHeard(c: Constants, v: Variables) 
+    requires v.WF(c)
+  {
+    forall idx, b| c.ValidLeaderIdx(idx) && v.leaders[idx].highestHeardBallot == Some(b)
+    :: (exists prom: Message ::
+          && prom.Promise? && prom in v.network.sentMsgs 
+          && prom.bal == idx
+          && prom.vbOpt == Some(VB(v.leaders[idx].value, b))
+      )
+  }
+
+  // certified self-inductive
+  // Acceptor updates its promised ballot based on a Prepare/Propose message carrying 
+  // that ballot
+  predicate AcceptorValidPromised(c: Constants, v: Variables)
+    requires v.WF(c)
+  {
+    forall idx, b | c.ValidAcceptorIdx(idx) && v.acceptors[idx].promised == Some(b)
+    :: (exists m: Message ::
+          && m in v.network.sentMsgs 
+          && (m.Promise? || m.Propose?)
+          && m.bal == b
+      )
+  }
+
+  // certified self-inductive
+  // Acceptor updates its acceptedVB based on a Propose message carrying that ballot 
+  // and value
+  predicate AcceptorValidAcceptedVB(c: Constants, v: Variables)
+    requires v.WF(c)
+  {
+    forall idx, val, bal | 
+      && c.ValidAcceptorIdx(idx) 
+      && v.acceptors[idx].acceptedVB == Some(VB(val, bal))
+    :: 
+      Propose(bal, val) in v.network.sentMsgs
   }
 
   predicate MessageInv(c: Constants, v: Variables) 
   {
     && v.WF(c)
     && ValidMessageSrc(c, v)
+    && LeaderValidHighestHeard(c, v)
+    && AcceptorValidPromised(c, v)
+    && AcceptorValidAcceptedVB(c, v)
   }
 
   lemma InitImpliesMessageInv(c: Constants, v: Variables)
@@ -39,7 +84,9 @@ module PaxosProof {
     requires MessageInv(c, v)
     requires Next(c, v, v')
     ensures MessageInv(c, v')
-  {}
+  {
+    // assert false;
+  }
 
 
   /***************************************************************************************
